progs64/proofmode_test.v
@@ -1,0 +1,187 @@
+Require Import VST.veric.juicy_base.
+Require Import VST.veric.mpred.
+Require Import VST.veric.env.
+Require Import VST.veric.lifting_expr.
+Require Import VST.veric.lifting.
+Require Import VST.veric.mapsto_memory_block.
+Require Import VST.veric.Clight_seplog.
+Require Import VST.veric.proofmode.
+Require Import VST.progs64.swap.
+Import Clight.
+Import Ctypesdefs.
+
+Definition fun_triple `{!VSTGS OK_ty Σ} OK_spec cs (P : list val → assert) f Q : Prop :=
+  forall ge args, P args -∗ stackframe_of' cs f (args ++ repeat Vundef (length (fn_temps f))) -∗
+    wp OK_spec (Build_genv ge cs) ⊤ f (fn_body f)
+       (frame_ret_assert (function_body_ret_assert (fn_return f) Q) (∃ lv, stackframe_of' cs f lv)).
+
+Section swap.
+
+Context `{VSTGS OK_ty Σ}.
+
+Theorem swap_correct Espec ge E f ix iy :
+  ⊢ temp _x (Vint ix) ∗ temp _y (Vint iy) ∗ temp _tmp Vundef -∗
+  wp Espec ge E f (fn_body f_swap)
+    (normal_ret_assert (temp _x (Vint iy) ∗ temp _y (Vint ix) ∗ ∃ v, temp _tmp v)).
+Proof.
+  iIntros "(Hx & Hy & Htmp)".
+  simpl.
+  wp_set; wp_temp; simpl.
+  wp_set; wp_temp; simpl.
+  wp_set; wp_temp; simpl.
+  iFrame.
+Qed.
+
+Theorem swap_fun Espec cs : fun_triple Espec cs (λ args, <affine> ⌜exists ix iy, args = [Vint ix; Vint iy]⌝) f_swap (λ _, emp).
+Proof.
+  iIntros (??) "(% & % & ->) S"; rewrite /stackframe_of' /=.
+  iDestruct "S" as "(_ & ? & ? & ? & _)".
+  wp_set; wp_temp; simpl.
+  wp_set; wp_temp; simpl.
+  wp_set; wp_temp; simpl.
+  iSplit; first done.
+  iExists [_; _; _]; simpl; iFrame.
+Qed.
+
+End swap.
+
+Require Import VST.veric.make_compspecs. (* deduplicate *)
+Require Import VST.veric.expr.
+Require Import VST.veric.val_lemmas.
+Require Import VST.floyd.mapsto_memory_block.
+Require Import VST.floyd.nested_field_lemmas.
+Require Import VST.floyd.field_at.
+Require Import VST.progs64.append.
+Transparent Archi.ptr64.
+
+Section append.
+
+Context `{VSTGS OK_ty Σ}.
+
+#[local] Instance CompSpecs : compspecs. make_compspecs prog. Defined.
+
+Definition t_struct_list := Tstruct _list noattr.
+
+Fixpoint listrep (sh: share)
+            (contents: list val) (x: val) : assert :=
+ match contents with
+ | h::hs =>
+              ∃ y:val,
+                ⎡data_at sh t_struct_list (h,y) x⎤ ∗ listrep sh hs y
+ | nil => ⌜x = nullval⌝ ∧ emp
+ end.
+
+Lemma listrep_isptr : forall sh l x, listrep sh l x ⊢ ⌜val_lemmas.is_pointer_or_null x⌝.
+Proof.
+  intros; destruct l; simpl.
+  - by iIntros "(-> & _)".
+  - iIntros "(% & H & _)".
+    rewrite data_at_isptr.
+    iDestruct "H" as "(% & _)"; destruct x; auto.
+Qed.
+
+Transparent peq.
+#[global] Arguments Pos.add : simpl nomatch.
+#[global] Arguments Pos.mul : simpl nomatch.
+#[global] Arguments Z.mul : simpl nomatch.
+#[global] Arguments Z.add : simpl nomatch.
+#[global] Arguments Z.div _ _ /.
+
+Definition list_body sh h y x :=
+  mapsto sh tint x h ∗ spacer sh 4 8 x ∗
+  mapsto sh (tptr t_struct_list) (offset_val 8 x) y.
+
+Lemma list_unfold : forall sh (h y x : val), data_at sh t_struct_list (h,y) x =
+  (⌜field_compatible t_struct_list [] x⌝ ∧ list_body sh h y x).
+Proof.
+  intros.
+  rewrite /data_at /field_at /at_offset /=.
+  apply andp_prop_eq1; first apply field_compatible_dec; intros Hcompat.
+  rewrite functional_base.isptr_offset_val_zero; last by destruct Hcompat.
+  rewrite data_at_rec_lemmas.data_at_rec_eq /=.
+  rewrite /fieldlist.field_offset_next /= /withspacer /at_offset /=.
+  rewrite functional_base.isptr_offset_val_zero; last by destruct Hcompat.
+  rewrite data_at_rec_lemmas.data_at_rec_eq /= -sep_assoc //.
+Qed.
+
+Theorem append_spec Espec lx ly : fun_triple Espec cenv_cs (λ args, ∃ x y, <affine> ⌜args = [x; y]⌝ ∗ listrep Ews lx x ∗ listrep Ews ly y)
+  f_append (λ r, ∃ z, <affine> ⌜r = Some z⌝ ∗ listrep Ews (lx ++ ly) z).
+Proof.
+  iIntros (??) "(% & % & -> & Hx & Hy) S"; rewrite /stackframe_of' /=.
+  iDestruct "S" as "(_ & Htx & Hty & Ht & Hu & _)".
+  wp_if.
+  wp_binop.
+  wp_temp.
+  destruct lx; simpl.
+  - iDestruct "Hx" as "(-> & _)".
+    wp_cast.
+    iNext; iSplit; first done; simpl.
+    wp_return.
+    iDestruct (listrep_isptr with "Hy") as %?.
+    wp_temp.
+    simpl.
+    iSplitL "Hy"; last by iExists [_; _; _; _]; iFrame.
+    rewrite /= /bind_ret /=.
+    by iFrame.
+  - iDestruct "Hx" as "(%tl & Hx & Htl)".
+    rewrite data_at_isptr; iDestruct "Hx" as "(% & Hx)".
+    destruct x; try contradiction.
+    wp_cast.
+    { simpl.
+      rewrite /sc_cmp /= /sc_cmp_ptr /=.
+      iApply valid_pointer_weak; iApply (data_at_valid_ptr with "Hx"); auto; simpl; lia. }
+    iNext; iSplit; first done; simpl.
+    wp_set; wp_temp; simpl.
+    rewrite list_unfold; iDestruct "Hx" as "(% & Hhd1 & Hspace & Htl1)".
+    wp_set. wp_load.
+    iDestruct (listrep_isptr with "Htl") as %?.
+    wp_field. wp_deref. wp_temp.
+    { by intros ->. }
+    reshape_seq.
+    iAssert (∃ t u a l', <affine> ⌜field_compatible t_struct_list [] t⌝ ∗ temp _t t ∗ temp _u u ∗
+      ⎡list_body Ews a u t⎤ ∗ listrep Ews l' u ∗
+      (listrep Ews (a :: l' ++ ly) t -∗ listrep Ews (v :: lx ++ ly) (Vptr b i))) with "[Ht Hu Hhd1 Hspace Htl1 Htl]"
+      as "(% & % & % & % & %Ht & Ht & Hu & Ht1 & Hl' & Hpre)".
+    { iFrame. simpl offset_val; iFrame; auto. }
+    iInduction l' as [|h' l'] "IH" forall (t u a Ht); simpl; wp_loop.
+    + iDestruct "Hl'" as "(-> & _)".
+      wp_if; wp_binop; wp_temp.
+      wp_cast.
+      iNext; iSplit; first done; simpl.
+      wp_break; simpl.
+      iDestruct (listrep_isptr with "Hy") as %Hy.
+      wp_store; wp_temp.
+      iSplit.
+      { iPureIntro; intros ?; simpl; done. }
+      iDestruct "Ht1" as "(Ht1 & ? & ?)".
+      destruct t; try (destruct Ht; contradiction).
+      wp_field. wp_deref. wp_temp.
+      wp_return. wp_temp; simpl.
+      iSplitR "Htx Hty Ht Hu"; last by iExists [_; _; _; _]; iFrame.
+      rewrite /= /bind_ret /=.
+      iSplit; first done; iExists _; iSplit; first done.
+      iApply "Hpre"; iFrame.
+      rewrite list_unfold; by iFrame.
+    + iDestruct "Hl'" as "(%tl' & Hh' & Hl')".
+      rewrite data_at_isptr; iDestruct "Hh'" as "(% & Hh')".
+      destruct u; try contradiction.
+      wp_if; wp_binop; wp_temp.
+      wp_cast.
+      { simpl.
+        rewrite /sc_cmp /= /sc_cmp_ptr /=.
+        iApply valid_pointer_weak; iApply (data_at_valid_ptr with "Hh'"); auto; simpl; lia. }
+      iNext; iSplit; first done; simpl.
+      wp_skip; simpl.
+      wp_set; wp_temp; simpl.
+      rewrite list_unfold; iDestruct "Hh'" as "(% & Hhd1 & Hspace & Htl1)".
+      wp_set. wp_load.
+      iDestruct (listrep_isptr with "Hl'") as %?.
+      wp_field. wp_deref. wp_temp.
+      { by intros ->. }
+      wp_skip; simpl.
+      iApply ("IH" with "[//] Hy [$] [$] [$] [$] [$] Hl'").
+      iIntros "H"; iApply "Hpre"; iFrame.
+      rewrite list_unfold; by iFrame.
+Qed.
+
+End append.
